Some work in parametric completeness proof.

SeparationLogic/Semantics.v
@@ -1,4 +1,6 @@
 Require Import Coq.Logic.Classical_Prop.
+Require Import Coq.Classes.RelationClasses.
+Require Import Coq.Relations.Relation_Definitions.
 Require Import Logic.lib.Coqlib.
 Require Import Logic.MinimunLogic.LogicBase.
 Require Import Logic.PropositionalLogic.Syntax.
@@ -31,11 +33,14 @@ Module DownwardsSemantics.
     {
       sat_sepcon: forall m x y,
         KRIPKE: M , m |= x * y <->
-                    exists m1 m2, join m1 m2 m /\ KRIPKE: M , m1 |= x /\ KRIPKE: M, m2 |= y;
+                    exists m1 m2, join m1 m2 m /\
+                                  KRIPKE: M , m1 |= x /\
+                                  KRIPKE: M, m2 |= y;
       sat_wand: forall m x y,
           KRIPKE: M , m |= x -* y <->
-                      forall m0 m1 m2, m0 <= m -> join m0 m1 m2 ->
-                                  KRIPKE: M , m1 |= x -> KRIPKE: M, m2 |= y
+                      forall m0 m1 m2,
+                        m0 <= m -> join m0 m1 m2 ->
+                        KRIPKE: M , m1 |= x -> KRIPKE: M, m2 |= y
 }.
 
 End DownwardsSemantics.
@@ -108,3 +113,152 @@ Class UnitarySemantics
       {kiSM: KripkeIntuitionisticSemantics L MD M SM}: Type :=
     sat_emp: forall (m: Kworlds M), KRIPKE: M, m |= emp <-> pre_unit m.
 
+Module FlatSemanticsModel.
+
+Import UnitarySeparationLanguage.
+
+Record frame: Type := {
+  underlying_set:> Type;
+  Korder: relation underlying_set; (* <= *)
+  Korder_preorder: PreOrder Korder;
+  kiM: KripkeIntuitionisticModel underlying_set :=
+         Build_KripkeIntuitionisticModel _ Korder Korder_preorder;
+  J: Join underlying_set;
+  SA: SeparationAlgebra underlying_set;
+  dSA: DownwardsClosedSeparationAlgebra underlying_set;
+  uSA: UpwardsClosedSeparationAlgebra underlying_set
+}.
+
+Infix "<=" := (Korder _): TheKripkeSemantics.
+
+Local Open Scope TheKripkeSemantics.
+
+Definition sem (f: frame) := sig (fun s: Ensemble f => forall x y, x <= y -> s y -> s x).
+
+Program Definition sem_and {F: frame} (X: sem F) (Y: sem F): sem F :=
+  fun x: F => X x /\ Y x.
+Next Obligation.
+  split.
+  + eapply (proj2_sig X); eauto.
+  + eapply (proj2_sig Y); eauto.
+Qed.
+
+Program Definition sem_or {F: frame} (X: sem F) (Y: sem F): sem F :=
+  fun x: F => X x \/ Y x.
+Next Obligation.
+  destruct H0; [left | right].
+  + eapply (proj2_sig X); eauto.
+  + eapply (proj2_sig Y); eauto.
+Qed.
+
+Program Definition sem_imp {F: frame} (X: sem F) (Y: sem F): sem F :=
+  fun x: F =>
+    forall y: F, y <= x -> X y -> Y y.
+Next Obligation.
+  revert H2; apply H0.
+  pose proof @PreOrder_Transitive _ _ (Korder_preorder F).
+  transitivity x; auto.
+Qed.
+
+Program Definition sem_true {F: frame}: sem F :=
+  fun x: F => True.
+
+Program Definition sem_false {F: frame}: sem F :=
+  fun x: F => False.
+
+Program Definition sem_sepcon {F: frame} (X: sem F) (Y: sem F): sem F :=
+  fun m: F =>
+    exists m1 m2, @join _ (J F) m1 m2 m /\ X m1 /\ Y m2.
+Next Obligation.
+  rename H0 into y1, H1 into y2.
+  destruct (@join_Korder_down _ _ _ (dSA F) _ _ _ _ H2 H) as [x1 [x2 [? [? ?]]]].
+  exists x1, x2.
+  split; [| split]; auto.
+  + eapply (proj2_sig X); eauto.
+  + eapply (proj2_sig Y); eauto.
+Qed.
+
+Program Definition sem_wand {F: frame} (X: sem F) (Y: sem F): sem F :=
+  fun m: F =>
+    forall m1 m2, @join _ (J F) m m1 m2 -> X m1 -> Y m2.
+Next Obligation.
+  destruct (@join_Korder_up _ _ _ (uSA F) _ _ _ _ m1 H1 H) as [m [? ?]].
+  + reflexivity.
+  + eapply (proj2_sig Y); [eauto |].
+    eapply H0; eauto.
+Qed.
+
+Program Definition sem_emp {F: frame}: sem F :=
+  fun m: F => @pre_unit _ (kiM F) (J F) m.
+Next Obligation.
+  unfold pre_unit in *.
+  intros.
+  destruct (@join_Korder_up _ _ _ (uSA F) _ _ _ _ n H1 H) as [m' [? ?]].
+  + reflexivity.
+  + specialize (H0 _ _ H2).
+    etransitivity; eauto.
+Qed.
+  
+Definition denotation {Var: Type} (F: frame) (eval: Var -> sem F): expr Var -> sem F :=
+  fix denotation (x: expr Var): sem F:=
+  match x with
+  | andp y z => sem_and (denotation y) (denotation z)
+  | orp y z => sem_or (denotation y) (denotation z)
+  | impp y z => sem_imp (denotation y) (denotation z)
+  | sepcon y z => sem_sepcon (denotation y) (denotation z)
+  | wand y z => sem_wand (denotation y) (denotation z)
+  | emp => sem_emp
+  | falsep => sem_false
+  | varp p => eval p
+  end.
+
+Section KripkeSemantics.
+Context (Var: Type).
+
+Record Kmodel : Type := {
+  underlying_frame :> frame;
+  Kvar: Var -> sem underlying_frame
+}.
+
+Record model: Type := {
+  underlying_model :> Kmodel;
+  elm: underlying_model
+}.
+
+Instance L: Language := UnitarySeparationLanguage.L Var.
+Instance MD: Model := Build_Model model.
+
+Instance kMD: KripkeModel MD :=
+  Build_KripkeModel _
+    Kmodel
+    (fun M => M)
+    (fun M m => Build_model M m).
+
+Existing Instances kiM J SA dSA uSA.
+
+Instance SM: Semantics L MD :=
+  Build_Semantics L MD
+   (fun M x => proj1_sig (denotation M (Kvar M) x) (elm M)).
+
+Instance kiSM (M: Kmodel): KripkeIntuitionisticSemantics L MD M SM.
+Proof.
+  apply Build_KripkeIntuitionisticSemantics.
+  + hnf; simpl; intros.
+    eapply (proj2_sig (denotation M (Kvar M) x)); eauto.
+  + split; auto.
+  + split; auto.
+  + split; auto.
+  + intros; simpl. auto.
+Defined.
+
+Definition Kmodel_Identical: Kmodel -> Prop := fun M =>
+  IdentityKripkeIntuitionisticModel (Kworlds M).
+
+Definition Kmodel_NoBranch: Kmodel -> Prop := fun M =>
+  NoBranchKripkeIntuitionisticModel (Kworlds M).
+
+Definition Kmodel_BranchJoin: Kmodel -> Prop := fun M =>
+  BranchJoinKripkeIntuitionisticModel (Kworlds M).
+
+End KripkeSemantics.
+End FlatSemanticsModel.
