SeparationLogic/Complete_Flat.v
@@ -3,6 +3,7 @@ Require Import Logic.lib.Coqlib.
 Require Import Logic.lib.Bijection.
 Require Import Logic.lib.Countable.
 Require Import Logic.MinimunLogic.LogicBase.
+Require Import Logic.MinimunLogic.MinimunLogic.
 Require Import Logic.PropositionalLogic.Syntax.
 Require Import Logic.SeparationLogic.Syntax.
 Require Import Logic.PropositionalLogic.KripkeSemantics.
@@ -25,16 +26,18 @@ Section Canonical_All.
 Context (Var: Type).
 Context (CV: Countable Var).
 
-Instance L: Language := SepLanguage.L Var.
-Instance nL: NormalLanguage L := PropositionalLanguage.nL Var.
-Instance pL: PropositionalLanguage L := PropositionalLanguage.pL Var.
-Instance G: ProofTheory L := IntuitionisticPropositionalLogic.G Var.
-Instance nG: NormalProofTheory L G := IntuitionisticPropositionalLogic.nG Var.
-Instance mpG: MinimunPropositionalLogic L G := IntuitionisticPropositionalLogic.mpG Var.
-Instance ipG: IntuitionisticPropositionalLogic L G := IntuitionisticPropositionalLogic.ipG Var.
-Instance MD: Model := KripkeSemantics.MD Var.
-Instance kMD: KripkeModel MD := KripkeSemantics.kMD Var.
-Instance kiM (M: Kmodel): KripkeIntuitionisticModel (Kworlds M):= KripkeSemantics.kiM Var M.
+Instance L: Language := SeparationLanguage.L Var.
+Instance nL: NormalLanguage L := SeparationLanguage.nL Var.
+Instance pL: PropositionalLanguage L := SeparationLanguage.pL Var.
+Instance G: ProofTheory L := SeparationLogic.G Var.
+Instance nG: NormalProofTheory L G := SeparationLogic.nG Var.
+Instance mpG: MinimunPropositionalLogic L G := SeparationLogic.mpG Var.
+Instance ipG: IntuitionisticPropositionalLogic L G := SeparationLogic.ipG Var.
+Instance MD: Model := FlatSemanticsModel.MD Var.
+Instance kMD: KripkeModel MD := FlatSemanticsModel.kMD Var.
+Check FlatSemanticsModel.kiM.
+Print Kmodel.
+Instance kiM (M: Kmodel): KripkeIntuitionisticModel (Kworlds M):= FlatSemanticsModel.kiM (underlying_frame M).
 Instance SM: Semantics L MD := KripkeSemantics.SM Var.
 Instance kiSM (M: Kmodel): KripkeIntuitionisticSemantics L MD M SM := KripkeSemantics.kiSM Var M.
 
